verified encoding stuff

LeanSAT/Encode/EncCNF.lean
@@ -3,6 +3,7 @@ import LeanSAT.Data.Cnf
 import LeanSAT.Data.ICnf
 import LeanSAT.Data.HashAssn
 import LeanSAT.Upstream.ToStd
+import LeanSAT.Model.Quantification
 
 open Std
 
@@ -10,156 +11,285 @@ namespace LeanSAT.Encode
 
 namespace EncCNF
 
-/-- State for an encoding -/
-structure State where
+/-- State for an encoding.
+
+We need to parameterize by literal type `L` (and variable `ν`),
+because otherwise we need to prove everywhere that clauses are "within range"
+ -/
+structure State (L ν : Type u) where
   nextVar : PNat
-  clauses : List (IClause)
-  names   : HashMap IVar String
-  varCtx  : String
-  conditionCtx : Array ILit
+  cnf : ICnf
+  vMap : ν → IVar
+  /-- we are currently assuming `¬ assumeVars` -/
+  assumeVars : Clause L
 
-namespace State
+/-- Lawfulness conditions on encoding state. -/
+structure LawfulState (L ν) extends State L ν where
+  cnfVarsLt : ∀ c ∈ cnf.data, ∀ l ∈ c.data, (LitVar.toVar l) < nextVar
+  vMapLt : ∀ v, vMap v < nextVar
+  vMapInj : vMap.Injective
 
-def new : State := ⟨1, [], HashMap.empty, "", #[]⟩
+instance : Coe (LawfulState L ν) (State L ν) := ⟨LawfulState.toState⟩
 
-instance : Inhabited State := ⟨new⟩
+def State.new (vars : PNat) (f : ν → IVar) : State L ν := {
+  nextVar := vars
+  cnf := #[]
+  vMap := f
+  assumeVars := #[]
+}
 
-def scramble (s : State) : IO State := do
-  let litsScrambled ← s.clauses.mapM fun ⟨lits⟩ => do
-    return ⟨← (IO.randPerm lits)⟩
-  let clausesScrambled ← IO.randPerm litsScrambled
-  return { s with clauses := clausesScrambled }
+def LawfulState.new (vars : PNat) (f : ν → IVar)
+      (fInj : f.Injective) (h : ∀ v, f v < vars) : LawfulState L ν := {
+  State.new vars f with
+  cnfVarsLt := by intro c hc _ _; simp [State.new] at hc
+  vMapLt := h
+  vMapInj := fInj
+}
 
-def toFormula : State → ICnf
-| {clauses, ..} => clauses.toArray
+def State.scramble (s : State L ν) : IO (State L ν) := do
+  let clauseScrambled ← s.cnf.mapM fun clause => do
+    return (← IO.randPerm clause.toList).toArray
+  let cnf := (← IO.randPerm clauseScrambled.toList).toArray
+  return { s with
+    cnf
+  }
 
-nonrec def toString : State → String
-| {clauses,names,nextVar, ..} => Id.run do
-  let mut acc := ""
-  for i in [0:nextVar] do
-    match names.find? (i.succPNat) with
-    | none => ()
-    | some name => acc := acc ++ s!"c {i} {name}\n"
-  acc ++ toString clauses
-
-instance : ToString State := ⟨toString⟩
-end State
+instance : ToString (State L ν) := ⟨toString ∘ State.cnf⟩
 
 end EncCNF
 
-@[reducible]
-def EncCNF := ExceptT String (StateM EncCNF.State)
+/-- Encoding monad.
+
+This requires quite a few invariants to be held.
+It receives and produces lawful states, and
+never decreases the `nextVar`.
+-/
+def EncCNF (L) [LitVar L ν] (α) :=
+  { sa : StateM (EncCNF.LawfulState L ν) α //
+    ∀ s, s.nextVar ≤ (sa s).2.nextVar }
 
 namespace EncCNF
 
-nonrec def run? (s : State) (e : EncCNF α) : Except String (α × State) := do
-  let (a,s) := e.run s
-  return (←a, s)
+variable {L} [LitVar L ν]
 
-nonrec def run! [Inhabited α] (s : State) (e : EncCNF α) : α × State :=
-  (run? s e).toOption.get!
+instance : Monad (EncCNF L) where
+  pure a := ⟨pure a, by simp [pure, StateT.pure]⟩
+  bind | ⟨sa,h⟩, f => ⟨bind sa (f · |>.1), by
+    intro s
+    simp [bind, StateT.bind]
+    split
+    next a s' hs' =>
+    apply Nat.le_trans (m := s'.nextVar)
+    · have := h s
+      rw [hs'] at this
+      exact this
+    · exact (f a).2 s'
+    ⟩
 
-nonrec def new? : EncCNF α → Except String (α × State)  := run? .new
-nonrec def new! [Inhabited α] : EncCNF α → α × State    := run! .new
-
-instance [Inhabited α] : Inhabited (EncCNF α) := ⟨do return default⟩
-
-def newCtx (name : String) (inner : EncCNF α) : EncCNF α := do
-  let oldState ← get
-  set {oldState with varCtx := oldState.varCtx ++ name}
+def newCtx (name : String) (inner : EncCNF L α) : EncCNF L α := do
   let res ← inner
-  let newState ← get
-  set {newState with varCtx := oldState.varCtx}
   return res
 
-def mkVar (name : String) : EncCNF IVar := do
-  let oldState ← get
-  set { oldState with
-    nextVar := oldState.nextVar + 1,
-    names := oldState.names.insert oldState.nextVar
-                (oldState.varCtx ++ name)}
-  return oldState.nextVar
-
-def mkTemp : EncCNF IVar := do
-  let oldState ← get
-  return ← mkVar ("tmp" ++ toString oldState.nextVar)
-
-def addClause (C : IClause) : EncCNF Unit := do
-  let oldState ← get
-  set { oldState with
-    clauses := (oldState.conditionCtx ++ C) :: oldState.clauses }
+def addClause (C : Clause L) : EncCNF L Unit :=
+  ⟨ fun {nextVar,cnf,vMap,assumeVars,cnfVarsLt,vMapLt,vMapInj} =>
+    ((), {
+      nextVar, vMap, assumeVars
+      vMapLt, vMapInj
+      cnf := cnf.addClause ((Clause.or assumeVars C).map _ vMap)
+      cnfVarsLt := by
+        intro c hc v hv
+        simp [Cnf.addClause, Clause.or, LitVar.map] at hc
+        cases hc
+        · apply cnfVarsLt; repeat assumption
+        · subst_vars; simp [Clause.map] at hv
+          rcases hv with ⟨a,_,rfl⟩ | ⟨a,_,rfl⟩
+          · simp [LitVar.map]; apply vMapLt
+          · simp [LitVar.map]; apply vMapLt
+    }),
+    by simp⟩
 
 /-- runs `e`, adding `ls` to each generated clause -/
-def unlessOneOf (ls : Array ILit) (e : EncCNF α) : EncCNF α := do
-  let oldState ← get
-  set { oldState with conditionCtx := oldState.conditionCtx ++ ls }
-  let res ← e
-  let newState ← get
-  set { newState with conditionCtx := oldState.conditionCtx }
-  return res
+def unlessOneOf (ls : Array L) (e : EncCNF L α) : EncCNF L α :=
+  ⟨ fun state =>
+    let oldAssumes := state.assumeVars
+    let newState := { state with
+      assumeVars := oldAssumes.or ls
+    }
+    let (res, newState) := e.1 newState
+    (res, {newState with
+      assumeVars := oldAssumes
+    }),
+    by intro s; simp; split; next a s' hs' =>
+      simp; have := hs' ▸ e.2 _; simpa using this⟩
 
-def assuming (ls : Array ILit) (e : EncCNF α) : EncCNF α :=
-  -- Literal negation here
+def assuming [LawfulLitVar L ν] (ls : Array L) (e : EncCNF L α) : EncCNF L α :=
   unlessOneOf (ls.map (- ·)) e
 
-structure IVarBlock (dims : List Nat) where
-  start : IVar
-  h_dims : dims.length > 0
+def blockAssn [BEq ν] [Hashable ν] (a : HashAssn L) : EncCNF L Unit :=
+  addClause (a.toLitArray.map (- ·))
 
-namespace IVarBlock
-
-instance : Inhabited (IVarBlock (x::xs)) where
-  default := {start := 1, h_dims := by simp [Nat.succ_pos]}
-
-@[reducible, inline, simp]
-def hdLen : IVarBlock ds → Nat
-| ⟨_, _⟩ =>
-  match ds with
-  | [] => by contradiction
-  | d::_ => d
-
-@[reducible, inline, simp]
-def elemTy : List Nat → Type
-  | [] => Empty
-  | [_] => IVar
-  | _::d'::ds' => IVarBlock (d'::ds')
-
-@[inline]
-def get (v : IVarBlock ds) (i : Fin v.hdLen)
-  : IVarBlock.elemTy ds
-  := match ds, v with
-  | [],         ⟨_    ,_⟩ => by contradiction
-  | [_],        ⟨start,_⟩ => ⟨start + i.val, Nat.add_pos_left start.property _⟩
-  | _::d'::ds', ⟨start,_⟩ =>
-    { start := ⟨start + (Nat.mul i ((d'::ds').foldl (· * ·) 1)), Nat.add_pos_left start.property _⟩
-      h_dims := by simp
-    }
-
-instance : GetElem (IVarBlock ds) Nat (IVarBlock.elemTy ds) (fun v i => i < v.hdLen) where
-  getElem v i h := v.get ⟨i,h⟩
-
-end IVarBlock
-
-def mkVarBlock (name : String) (dims : List Nat) (h : dims.length > 0 := by simp)
-  : EncCNF (IVarBlock dims) := do
-  let state ← get
-  let start := state.nextVar
-  gen dims name
-  return ⟨start, h⟩
-where gen (dims : List Nat) (pref : String) : EncCNF Unit := do
-  match dims with
-  | [] =>
-    let _ ← mkVar pref
-  | d::ds =>
-    for i in [0:d] do
-      gen ds s!"{pref}[{i}]"
-
-def mkTempBlock (dims : List Nat) (h : dims.length > 0 := by simp)
-  : EncCNF (IVarBlock dims) := do
-  return ← mkVarBlock ("tmp" ++ toString (← get).nextVar) dims h
-
-def blockAssn (a : HashAssn ILit) : EncCNF Unit := addClause (a.toLitArray.map (- ·))
-
-def addAssn (a : HashAssn ILit) : EncCNF Unit := do
+def addAssn [BEq ν] [Hashable ν] (a : HashAssn L) : EncCNF L Unit := do
   for l in a.toLitArray do
     addClause #[l]
+
+
+/-! ### Establishing interpretations of EncCNF -/
+
+namespace LawfulState
+
+/-- Thanks to `vInjLt` we know `V` is `Fintype`. -/
+noncomputable def fintype (s : LawfulState L ν) : Fintype ν :=
+  Fintype.ofInjective (β := Fin s.nextVar)
+    (fun v => ⟨s.vMap v, s.vMapLt ..⟩)
+    (by intro v1 v2 h
+        apply s.vMapInj
+        simpa [PNat.val, ← Subtype.ext_iff] using h)
+
+/-- The interpretation of an `EncCNF` state is the
+formula's interpretation, but with all temporaries
+existentially quantified away.
+-/
+noncomputable def interp (s : LawfulState L ν) : Model.PropFun ν :=
+  let φ := s.cnf.toPropFun
+  have := s.fintype
+  φ.invImage ⟨s.vMap, s.vMapInj⟩ Finset.univ
+
+end LawfulState
+
+
+/-! ### Temporaries -/
+
+def WithTemps (L n) := L ⊕ Fin n × Bool
+instance : LitVar (WithTemps L n) (ν ⊕ Fin n) where
+  negate | Sum.inl l => Sum.inl (LitVar.negate l)
+         | Sum.inr (i,p) => Sum.inr (i,!p)
+  mkPos | Sum.inl v => Sum.inl (LitVar.mkPos v)
+        | Sum.inr v => Sum.inr (v,true)
+  mkNeg | Sum.inl v => Sum.inl (LitVar.mkNeg v)
+        | Sum.inr v => Sum.inr (v,false)
+  toVar | Sum.inl l => Sum.inl (LitVar.toVar l)
+        | Sum.inr (i,_) => Sum.inr i
+  polarity | Sum.inl l => LitVar.polarity l
+           | Sum.inr (_,p) => p
+
+instance [LawfulLitVar L ν] : LawfulLitVar (WithTemps L n) (ν ⊕ Fin n) where
+  toVar_negate := by intro l; cases l <;> simp [LitVar.toVar]
+  toVar_mkPos := by intro v; cases v <;> simp [LitVar.toVar]
+  toVar_mkNeg := by intro v; cases v <;> simp [LitVar.toVar]
+  polarity_negate := by intro l; cases l <;> simp [LitVar.polarity]
+  polarity_mkPos := by intro v; cases v <;> simp [LitVar.polarity]
+  polarity_mkNeg := by intro v; cases v <;> simp [LitVar.polarity]
+  ext := by
+    intro l1 l2 h1 h2
+    cases l1 <;> cases l2
+      <;> simp [LitVar.toVar, LitVar.polarity] at h1 h2
+      <;> congr
+      <;> ext
+    repeat simp only [*]
+
+def State.withTemps (s : State L ν) : State (WithTemps L n) (ν ⊕ Fin n) where
+  nextVar := ⟨s.nextVar + n, by simp⟩
+  cnf := s.cnf
+  vMap := fun | Sum.inl v => s.vMap v | Sum.inr i => ⟨s.nextVar + i, by simp⟩
+  assumeVars := s.assumeVars.map _ (Sum.inl ·)
+
+@[simp] theorem State.cnf_withTemps (s : State L ν) :
+    (State.withTemps s (n := n)).cnf = s.cnf
+  := by simp [State.withTemps]
+
+def LawfulState.withTemps (s : LawfulState L ν)
+  : LawfulState (WithTemps L n) (ν ⊕ Fin n) where
+  toState := s.toState.withTemps
+  cnfVarsLt := by
+    simp [State.withTemps]
+    intro c hc l hl
+    apply Nat.lt_of_lt_of_le
+    · exact s.cnfVarsLt c hc l hl
+    · simp; apply Nat.le_add_right
+  vMapLt := by
+    simp [State.withTemps]
+    constructor
+    · intro v; apply Nat.lt_of_lt_of_le
+      · apply s.vMapLt
+      · simp; apply Nat.le_add_right
+    · intro a; apply (PNat.mk_lt_mk ..).mpr; simp
+  vMapInj := by
+    intro v1 v2
+    simp [State.withTemps]
+    cases v1 <;> cases v2 <;> simp
+    · apply s.vMapInj
+    · intro h; have := h ▸ s.vMapLt _; simp [← PNat.coe_lt_coe] at this
+    · intro h; have := h.symm ▸ s.vMapLt _; simp [← PNat.coe_lt_coe] at this
+    · rw [Subtype.mk_eq_mk]
+      intro h
+      apply Fin.eq_of_veq; apply Nat.add_left_cancel h
+
+def State.withoutTemps (vMap : ν → IVar) (assumeVars : Array L) (s : State (WithTemps L n) (ν ⊕ Fin n)) : State L ν where
+  nextVar := s.nextVar
+  cnf := s.cnf
+  vMap := vMap
+  assumeVars := assumeVars
+
+@[simp] theorem State.vMap_withoutTemps (s : State _ _) :
+    (State.withoutTemps (L := L) (ν := ν) (n := n) vm av s).vMap = vm
+  := by simp [State.withoutTemps]
+
+@[simp] theorem State.assumeVars_withoutTemps (s : State _ _) :
+    (State.withoutTemps (L := L) (ν := ν) (n := n) vm av s).assumeVars = av
+  := by simp [State.withoutTemps]
+
+def LawfulState.withoutTemps (s : LawfulState (WithTemps L n) (ν ⊕ Fin n))
+    (vMap : ν → IVar) (vMapLt : ∀ v, vMap v < s.nextVar) (vMapInj : vMap.Injective)
+    (assumeVars : Array L)
+    : LawfulState L ν where
+  toState := s.toState.withoutTemps vMap assumeVars
+  cnfVarsLt := by
+    simp [State.withoutTemps]
+    intro c hc l hl
+    apply Nat.lt_of_lt_of_le
+    · exact s.cnfVarsLt c hc l hl
+    · simp
+  vMapLt := by
+    simp [State.withoutTemps]
+    apply vMapLt
+  vMapInj := by
+    intro v1 v2
+    simp [State.withoutTemps]
+    apply vMapInj
+
+@[simp] theorem LawfulState.vMap_withoutTemps (s : LawfulState (WithTemps L n) (ν ⊕ Fin n))
+    {vMap : ν → IVar} {vMapLt : ∀ v, vMap v < s.nextVar} {vMapInj : vMap.Injective}
+    : (LawfulState.withoutTemps s vMap vMapLt vMapInj av).vMap = vMap
+  := by simp [LawfulState.withoutTemps]
+
+@[simp] theorem LawfulState.assumeVars_withoutTemps (s : LawfulState (WithTemps L n) (ν ⊕ Fin n))
+    {vMap : ν → IVar} {vMapLt : ∀ v, vMap v < s.nextVar} {vMapInj : vMap.Injective}
+    : (LawfulState.withoutTemps s vMap vMapLt vMapInj av).assumeVars = av
+  := by simp [LawfulState.withoutTemps]
+
+def nextVar_mono_of_eq {e : EncCNF L α} (h : e.1 s = (a, s')) :
+    s.nextVar ≤ s'.nextVar := by
+  have := h ▸ e.2 s
+  exact this
+
+def withTemps (n) (e : EncCNF (WithTemps L n) α) : EncCNF L α :=
+  ⟨ fun s =>
+    let vMap := s.vMap
+    let vMapInj := s.vMapInj
+    let assumeVars := s.assumeVars
+    match h : e.1 s.withTemps with
+    | (a,s') =>
+    (a, s'.withoutTemps vMap (by
+        intro v; simp; apply Nat.lt_of_lt_of_le (m := s.nextVar)
+        · apply s.vMapLt
+        · have := e.nextVar_mono_of_eq h
+          apply Nat.le_trans (m := s.nextVar + n)
+          · simp
+          · exact (PNat.coe_le_coe ..).mp this
+      ) vMapInj assumeVars)
+  , by simp [LawfulState.withoutTemps, State.withoutTemps]
+       intro s; split; simp; have := e.nextVar_mono_of_eq ‹_›
+       simp [LawfulState.withTemps, State.withTemps] at this
+       apply Nat.le_trans (m := s.nextVar + n)
+       · apply Nat.le_add_right
+       · exact (PNat.coe_le_coe ..).mp this⟩
